README.md
@@ -18,21 +18,21 @@ Dependencies
 
 The development version of Katamaran has the following lower bounds:
 ```
-coq            >= 8.17
+coq            >= 8.18
 coq-equations  >= 1.3
-coq-iris       >= 4.1
-coq-stdpp      >= 1.8
+coq-iris       >= 4.2
+coq-stdpp      >= 1.10
 ```
-and has also been tested with coq 8.18.
+and has also been tested with coq 8.19.
 
 ### Using opam
 
 An easy way to setup your system is to create a fresh opam switch, pin the Coq and Iris versions and install equations (stdpp will be installed as a dependency of Iris):
 ```
-opam switch create katamaran ocaml-base-compiler.4.14.1
+opam switch create katamaran ocaml-base-compiler.4.14.2
 opam repo add coq-released https://coq.inria.fr/opam/released
-opam pin add coq 8.17.1
-opam pin add coq-iris 4.1.0
+opam pin add coq 8.18.0
+opam pin add coq-iris 4.2.0
 opam install coq-equations
 ```
 
